# 09.01.2023

$$
\vec{EJ} \begin{pmatrix} 0 - 0 \\ -4 - 0 \\ 3 - 5 \end{pmatrix} \; = \begin{pmatrix} 0 \\ -4 \\ -2 \end{pmatrix} \;
$$

$$
\vec{FJ} \begin{pmatrix} 0 - 0 \\ 4 - 0 \\ 3 - 5 \end{pmatrix} \; = \begin{pmatrix} 0  \\ 4 \\ -2 \end{pmatrix} \;
$$

$$
\vec{HK} \begin{pmatrix} -10 - (-10) \\ -4 - 0 \\ 3 - 5 \end{pmatrix} \; = \begin{pmatrix} 0  \\ -4 \\ -2 \end{pmatrix} \;
$$

$$
\vec{GK} \begin{pmatrix} -10 - (-10) \\ 4 - 0 \\ 3 - 5 \end{pmatrix} \; = \begin{pmatrix} 0  \\ 4 \\ -2 \end{pmatrix} \;
$$

$$
\vec{JK} \begin{pmatrix} 0 - (-10) \\ 0 - 0 \\ 5 - 5 \end{pmatrix} \; = \begin{pmatrix} -10 \\ 0 \\ 0 \end{pmatrix} \;
$$
